Formalized permutation

QuickSortInLean/Permutation.lean
@@ -1,50 +1,262 @@
-class Interp (n : Nat) (α : Type) where
-  interp (self : α) : Fin n → Fin n
+import QuickSortInLean.QuickSort
+import Std.Data.Option.Basic
+import Std.Data.Fin.Basic
+import Std.Data.Array.Lemmas
 
-structure Transposition (n : Nat) where
-  i : Fin n
-  j : Fin n
+-- Reflexive and transitive closure of arr ⇒ arr.swap i j
+inductive permuted : Array α → Array α → Type where
+  | refl : permuted arr arr
+  | step {arr arr'} (i j : Fin arr.size) : permuted (arr.swap i j) arr' → permuted arr arr'
 
-def Transposition.interp (t : Transposition n) : Fin n → Fin n
-  | k =>
-    if k = t.i then t.j
-    else if k = t.j then t.i
-    else k
+-- theorem permuted_trans : permuted arr arr' → permuted arr' arr'' → permuted arr arr'' := by
+--   intro p
+--   induction p with
+--   | refl => intro; assumption
+--   | step _ ih =>
+--     intro q
+--     exact .step (ih q)
 
-instance : Interp n (Transposition n) where
-  interp := Transposition.interp
+-- NOTE: somehow we need to write ∃_ : permuted arr arr', True instead of permuted arr arr'.
+-- Otherwise, split tactic will not work.
+theorem partition'_permutation [Ord α] :
+  (partition' (arr : Array α) i j last ij jl la).2 = arr' → ∃_ : permuted arr arr', True := by
+  unfold partition'
+  split <;> simp [dbgTraceIfShared]
+  case inl jl =>
+    split
+    -- | .lt | .eq
+    case h_1 | h_2 =>
+      intro eq
+      let ⟨ih, _⟩ := partition'_permutation eq
+      exact ⟨.step _ _ ih, trivial⟩
+    -- | .gt
+    case h_3 =>
+      intro eq
+      exact partition'_permutation eq
+  case inr _ =>
+    intro eq
+    rw [←eq]
+    exact ⟨.step _ _ .refl, trivial⟩
+termination_by partition'_permutation α arr i j last ij jl la result ord => last - j
 
-abbrev Permutation (n : Nat) := List (Transposition n)
+theorem partition_permutation [Ord α] :
+  (partition (arr : Array α) first last jl la).2 = arr' → ∃_ : permuted arr arr', True := by
+    simp [partition]
+    exact partition'_permutation
 
-def Permutation.interp (p : Permutation n) : Fin n → Fin n :=
+-- TODO: It's really hard to see through the definition of quickSort'.
+theorem quickSort'_permutation [Ord α] :
+  (quickSort' (arr : Array α) first last la).val = arr' → ∃_ : permuted arr arr', True := by
+  sorry
+
+theorem quickSort_permutation [Ord α] :
+  (quickSort (arr : Array α)) = arr' → ∃_ : permuted arr arr', True := by
+  simp [quickSort]
+  split
+  case inl => exact quickSort'_permutation
+  case inr =>
+    intro eq
+    rw [eq]
+    exact ⟨.refl, trivial⟩
+
+def isInv (f : α → β) (g : β → α) :=
+  (∀ x, g (f x) = x) ∧ (∀ y, f (g y) = y)
+
+def invertible (f : α → β) := ∃g, isInv f g
+
+theorem invertible_id : invertible (id : α → α) := by
+  have : isInv (id : α → α) id := by
+    apply And.intro
+    . intro x
+      simp
+    . intro y
+      simp
+  exact ⟨id, this⟩
+
+def permuted.to_map (p : permuted arr arr') : Fin arr.size → Fin arr'.size :=
   match p with
-  | [] => id
-  | t :: ts => t.interp ∘ Permutation.interp ts
+  | .refl => id
+  | .step i j p' => fun k =>
+    have h : arr.size = (arr.swap i j).size := by simp
+    let k' :=
+      if k.val = i.val then j
+      else if k.val = j.val then i
+      else k
+    p'.to_map (k'.cast h)
 
-instance : Interp n (Permutation n) where
-  interp := Permutation.interp
-
-notation:max " 〚 " x " 〛 " => Interp.interp x
-infix:60 " ↔ " => Transposition.mk
-
--- #check 〚[0 ↔ 1, 3 ↔ 5]〛
-
-theorem Permutation.interp_id : (〚([] : Permutation n)〛 : Fin n → Fin n)= id :=
-  rfl
-
-theorem Permutation.interp_cons
-  (t : Transposition n) (ts : Permutation n)
-  : 〚(t :: ts)〛 = 〚t〛 ∘ (〚ts〛 : Fin n → Fin n) := rfl
-
-theorem Permutation.homomorphism :
-  ∀ (p q : Permutation n), (〚p ++ q〛 : Fin n → Fin n) = 〚p〛 ∘ 〚q〛 := by
-  intro p
+theorem permuted_size (p : permuted arr arr') : arr'.size = arr.size := by
   induction p with
-  | nil =>
-    intro q
-    simp [Permutation.interp_id]
-    rfl
-  | cons t ts ih =>
-    intro q
-    simp [Permutation.interp, Permutation.interp_cons, ih]
-    rfl
+  | refl => rfl
+  | step _ _ _ ih =>
+    simp at ih
+    exact ih
+
+theorem Fin.cast_eq_val {n m : Nat} (h : n = m) (i : Fin n) : (i.cast h).val = i.val := by
+  simp [Fin.cast]
+
+theorem Fin.eq_ite {n : Nat} (i j : Fin n) :
+  (if j.val = i.val then j else i) = i := by
+  cases Nat.decEq j.val i.val with
+  | isFalse h => simp [*]
+  | isTrue h => simp [*, Fin.eq_of_val_eq h]
+
+theorem permuted_map_invertible (p : permuted arr1 arr2) : invertible p.to_map := by
+  induction p with
+  | refl => simp [permuted.to_map, invertible_id]
+  | @step arr3 arr4 i j p ih =>
+    have size_s3 : (arr3.swap i j).size = arr3.size := by simp
+    let ⟨f', ⟨h1, h2⟩⟩ := ih
+    let f := permuted.to_map (permuted.step i j p)
+    show invertible f
+    let g := fun (k : Fin arr4.size) =>
+      let k := (f' k).cast size_s3
+      -- let k := (f' (f (k.cast size_43))).cast size_s3
+      if k.val = i.val then j
+      else if k.val = j.val then i
+      else k
+    have gf : ∀x, g (f x) = x := by
+      intro x
+      simp (config := {zeta := false}) [f, permuted.to_map]
+      cases Nat.decEq x.val i.val with
+      | isFalse nxi =>
+        cases Nat.decEq x.val j.val with
+        | isFalse nxj =>
+          simp (config := {zeta := false}) [nxi, nxj, g]
+          rw [h1]
+          simp [Fin.cast, nxi, nxj]
+        | isTrue xj =>
+          simp (config := {zeta := false}) [nxi, xj, Fin.eq_ite, g]
+          rw [h1]
+          simp [Fin.cast]
+          exact Fin.eq_of_val_eq xj.symm
+      | isTrue xi =>
+        simp (config := {zeta := false}) [xi, g]
+        rw [h1]
+        simp [Fin.cast, Fin.eq_ite]
+        exact Fin.eq_of_val_eq xi.symm
+    have fg : ∀y, f (g y) = y := by
+      intro y
+      simp (config := {zeta := false}) [g]
+      let k : Fin arr3.size := (f' y).cast size_s3
+      show f (if k.val = i.val then j else if k.val = j.val then i else k) = y
+      cases Nat.decEq k.val i.val with
+      | isFalse nki =>
+        cases Nat.decEq k.val j.val with
+        | isFalse nkj =>
+          simp [nki, nkj, permuted.to_map]
+          -- Consective Fin.cast cancel each other
+          show p.to_map (f' y) = y
+          apply h2
+        | isTrue kj =>
+          simp [nki, kj, permuted.to_map,Fin.eq_ite]
+          have : j = k := Fin.eq_of_val_eq kj.symm
+          simp [this]
+          show permuted.to_map p (f' y) = y
+          apply h2
+      | isTrue ki =>
+        simp [ki, permuted.to_map, Fin.eq_ite]
+        have : i = k := Fin.eq_of_val_eq ki.symm
+        simp [this]
+        show permuted.to_map p (f' y) = y
+        apply h2
+    exact ⟨g, ⟨gf, fg⟩⟩
+
+theorem Option.sum_inj {a b : α} : some a = some b → a = b := by simp
+
+theorem getElem?_some_getElem (arr : Array α) (i : Nat) (eq : arr[i]? = some v) :
+  ∃h : i < arr.size, arr[i] = v := by
+  simp [getElem?] at eq
+  cases Nat.decLt i arr.size with
+  | isFalse h => simp [h] at eq
+  | isTrue h =>
+    simp [h] at eq
+    exact ⟨h, eq⟩
+
+theorem Array.eq_get_swap_left (arr : Array α) (i j : Fin arr.size) (h : arr.size = (arr.swap i j).size) :
+  arr[i] = (arr.swap i j)[j.cast h] := by
+  show arr[i] = (arr.swap i j)[(j.cast h).val]
+  have : (arr.swap i j)[(j.cast h).val]? = some arr[i.val] := by
+    rw [Array.get?_swap arr i j (j.cast h).val, Fin.cast_eq_val]
+    simp
+  let ⟨_, eq⟩ := getElem?_some_getElem _ _ this
+  simp [*]
+
+theorem Array.eq_get_swap_right (arr : Array α) (i j : Fin arr.size) (h : arr.size = (arr.swap i j).size) :
+  arr[j] = (arr.swap i j)[i.cast h] := by
+  show arr[j] = (arr.swap i j)[(i.cast h).val]
+  have : (arr.swap i j)[(i.cast h).val]? = some arr[j.val] := by
+    rw [Array.get?_swap arr i j (i.cast h).val, Fin.cast_eq_val]
+    simp
+    intro eq
+    have : j = i := Fin.eq_of_val_eq eq
+    rw [this]
+  let ⟨_, eq⟩ := getElem?_some_getElem _ _ this
+  simp [*]
+
+theorem Array.eq_get_swap_neq (arr : Array α) (i j k : Fin arr.size) (h : arr.size = (arr.swap i j).size) :
+  i ≠ k → j ≠ k → arr[k] = (arr.swap i j)[k.cast h] := by
+  intro ik jk
+  have ikv : i.val ≠ k.val := by
+    intro eq
+    exact ik <| Fin.eq_of_val_eq eq
+  have jkv : j.val ≠ k.val := by
+    intro eq
+    exact jk <| Fin.eq_of_val_eq eq
+  show arr[k] = (arr.swap i j)[(k.cast h).val]
+  have : (arr.swap i j)[(k.cast h).val]? = some arr[k.val] := by
+    rw [Array.get?_swap arr i j (k.cast h).val, Fin.cast_eq_val]
+    simp [ikv, jkv, getElem?, k.isLt]
+  let ⟨_, eq⟩ := getElem?_some_getElem _ _ this
+  simp [*]
+
+theorem permuted_map_index (p : permuted arr1 arr2) (k : Fin arr1.size) :
+  arr1[k] = arr2[p.to_map k] := by
+  induction p with
+  | refl => simp [permuted.to_map]
+  | @step arr3 arr4 i j p ih =>
+    simp [permuted.to_map]
+    simp at ih
+    split
+    case step.inl eq =>
+      have : arr3[k.val] = arr3[i.val] := by simp [eq]
+      rw [this]
+      have : arr3.size = (arr3.swap i j).size := by simp
+      rw [←ih]
+      exact Array.eq_get_swap_left arr3 i j this
+    case step.inr neq =>
+      split
+      case inl eq =>
+        have : arr3[k.val] = arr3[j.val] := by simp [eq]
+        rw [this]
+        have : arr3.size = (arr3.swap i j).size := by simp
+        rw [←ih]
+        exact Array.eq_get_swap_right arr3 i j this
+      case inr neq' =>
+        have : arr3.size = (arr3.swap i j).size := by simp
+        rw [←ih]
+        have neq : i ≠ k := by
+          intro eq
+          apply neq
+          simp [eq]
+        have neq' : j ≠ k := by
+          intro eq
+          apply neq'
+          simp [eq]
+        exact Array.eq_get_swap_neq arr3 i j k this neq neq'
+
+theorem permuted_map_index_invertible {arr arr' : Array α} (p : permuted arr arr') :
+  ∃(f : Fin arr.size → Fin arr'.size),
+    invertible f ∧ (∀(i : Fin arr.size), arr[i] = arr'[f i]) := by
+  exists p.to_map
+  apply And.intro
+  . exact permuted_map_invertible p
+  . intro i
+    exact permuted_map_index p i
+
+theorem quickSort_map_index_invertible {arr arr' : Array α} [Ord α] :
+  quickSort arr = arr' →
+  ∃f : Fin arr.size → Fin arr'.size,
+    invertible f ∧ (∀i : Fin arr.size, arr[i] = arr'[f i]) := by
+  intro eq
+  let ⟨p, _⟩ := quickSort_permutation eq
+  exact permuted_map_index_invertible p
